CpcMini/Proofs/TypePreservation.lean
@@ -160,11 +160,12 @@ theorem generic_apply_subterms_non_none
   rcases typeof_apply_non_none_cases hApply with ⟨A, B, hF, hX, hA, hB⟩
   constructor
   · unfold term_has_non_none_type
-    cases hF with
-    | inl hF =>
-        rw [hF]
-        simp
-    | inr hF =>
+    rcases hF with hF | hF | hF
+    · rw [hF]
+      simp
+    · rw [hF]
+      simp
+    ·
         rw [hF]
         simp
   · unfold term_has_non_none_type
